template-coq/theories/utils.v
@@ -117,9 +117,17 @@ Proof.
       discriminate.
 Qed.
 
+Lemma uip_bool (b1 b2 : bool) (p q : b1 = b2) : p = q.
+Proof.
+  destruct q. apply Eqdep_dec.UIP_refl_bool.
+Qed.
+
 Ltac tas := try assumption.
 Ltac tea := try eassumption.
 
 Axiom todo : String.string -> forall {A}, A.
 Ltac todo s := exact (todo s).
 Extract Constant todo => "fun s -> failwith (String.concat """" (List.map (String.make 1) s))".
+
+
+Coercion is_left A B (u : {A} + {B}) := match u with left _ => true | _ => false end.
